wip

theories/hoare.v
@@ -18,31 +18,31 @@ Unset Printing Implicit Defensive.
 Local Open Scope classical_set_scope.
 Local Open Scope monae_scope.
 
-Record hoare T U : Type := mk_hoare {
+Record prepost T U : Type := mk_prepost {
   pre : set T ;
   post : T -> U -> set T }.
-Arguments mk_hoare {T U} (pre post).
+Arguments mk_prepost {T U} (pre post).
 Arguments pre {T U} (_ _).
 Arguments post {T U} (_ _ _).
 
 Module Hoare.
-Definition hoare_ret {T} {U : UU0} (x : U) : @hoare T U :=
-  mk_hoare [set: T] (fun s y s' => (x = y) /\ (s = s')).
+Definition prepost_ret {T} {U : UU0} (x : U) : @prepost T U :=
+  mk_prepost [set: T] (fun s y s' => (x = y) /\ (s = s')).
 
-Definition hoare_bind {T} {U V}
-    (m : hoare T U) (k : U -> hoare T V) : hoare T V := mk_hoare
+Definition prepost_bind {T} {U V}
+    (m : prepost T U) (k : U -> prepost T V) : prepost T V := mk_prepost
     (fun s => pre m s /\ (forall x, post m s x `<=` pre (k x)))
     (fun s x s2 => exists y s', post m s y s' /\ post (k y) s' x s2).
 
 Section hm.
 Context (T : UU0).
-Let ret := @hoare_ret T.
-Let bind := @hoare_bind T.
+Let ret := @prepost_ret T.
+Let bind := @prepost_bind T.
 
 Let right_neutral : BindLaws.right_neutral bind ret.
 Proof.
 move=> A [pr po].
-rewrite /bind /ret /hoare_bind /hoare_ret/=; congr mk_hoare.
+rewrite /bind /ret /prepost_bind /prepost_ret/=; congr mk_prepost.
 - by apply/seteqP; split => // s [].
 - apply/eq3_fun => s a s''.
   under eq2_exists do rewrite andA.
@@ -51,8 +51,8 @@ Qed.
 
 Let left_neutral : BindLaws.left_neutral bind ret.
 Proof.
-move=> A B a f; rewrite /bind /ret /hoare_bind /hoare_ret/=.
-move fa : (f a) => [pr po]; congr mk_hoare.
+move=> A B a f; rewrite /bind /ret /prepost_bind /prepost_ret/=.
+move fa : (f a) => [pr po]; congr mk_prepost.
 - apply/funext=> s; rewrite andTP; apply/propext; split.
   + by move=> /(_ a s); rewrite fa/=; exact.
   + by move=> prs _ _ [<- <-]; rewrite fa.
@@ -65,8 +65,8 @@ Qed.
 
 Let assoc : BindLaws.associative bind.
 Proof.
-move=> A B C m f g; rewrite /bind /ret /hoare_bind /hoare_ret/=.
-case: m => prA poA/=; congr mk_hoare.
+move=> A B C m f g; rewrite /bind /ret /prepost_bind /prepost_ret/=.
+case: m => prA poA/=; congr mk_prepost.
 - apply/funext=> s; apply/propext; split.
   + move=> [[prAs poApre postpre]].
     split => // a s1 sas1; split=> [|b s2 s'bs2].
@@ -86,7 +86,7 @@ case: m => prA poA/=; congr mk_hoare.
   by under [in RHS]eq2_exists do rewrite andA.
 Qed.
 
-HB.instance Definition _ := isMonad_ret_bind.Build (hoare T)
+HB.instance Definition _ := isMonad_ret_bind.Build (prepost T)
   left_neutral right_neutral assoc.
 
 End hm.
@@ -95,30 +95,30 @@ End Hoare.
 
 HB.export Hoare.
 
-HB.about hoare.
+HB.about prepost.
 
 HB.mixin Record isMonadHoare
 (T : UU0) (N : monad)
 (ST : stateRunMonad T N)
   (M : Type -> Type) of Monad M := {
-  valid_hoare : forall U : UU0, M U -> ST U -> Prop ;
+  valid_prepost : forall U : UU0, M U -> ST U -> Prop ;
   valid_ret : forall (U : UU0) (x : U),
-    valid_hoare U (Ret x) (Ret x) ;
+    valid_prepost U (Ret x) (Ret x) ;
   valid_bind : forall (U V : UU0) (h : M U) (m : ST U)
       (h' : U -> M V) (k : U -> ST V),
-    valid_hoare U h m ->
-    (forall x, valid_hoare V (h' x) (k x)) ->
-    valid_hoare V (h >>= h') (m >>= k)
+    valid_prepost U h m ->
+    (forall x, valid_prepost V (h' x) (k x)) ->
+    valid_prepost V (h >>= h') (m >>= k)
 }.
 
 #[short(type=hoareMonad)]
 HB.structure Definition MonadHoare (T : UU0) (N : monad) (ST : stateRunMonad T N) :=
   {M of isMonadHoare T N ST M & isMonad M & isFunctor M}.
 
-Arguments valid_hoare {T N ST M U} _ _ : rename.
+Arguments valid_prepost {T N ST M U} _ _ : rename.
 
 Notation "{{ pre }} prog {{ post }}" :=
-  (valid_hoare (mk_hoare pre post) prog)
+  (valid_prepost (mk_prepost pre post) prog)
   (at level 0,
    format "'[' {{  pre  }} '/ ' prog '/ ' {{  post  }} ']'").
 
@@ -127,25 +127,23 @@ From monae Require Import monad_model monad_transformer.
 Module HoareModel.
 Section vld_s.
 Context {T : UU0}.
- (* {ST : stateRunMonad T }. *)
-Abbreviation HT := (hoare T).
+Abbreviation HT := (prepost T).
 Abbreviation ST := (stateT T option_monad).
-
+(* Context {N : monad} {ST : stateRunMonad T N}. *)
 Definition valid {U : UU0} (h : HT U) (m : ST U) : Prop :=
   forall s, pre h s ->
     (forall a s', runStateT m s = Ret (a, s') -> post h s a s').
 
-Lemma valid_ret : forall U (x : U), valid (hoare_ret x) (Ret x) .
+Lemma valid_ret : forall U (x : U), valid (prepost_ret x) (Ret x) .
 Proof. by move=> U u t /= P u' t'; rewrite runStateTret; case. Qed.
 
 Lemma valid_bind : forall U V (h : HT U) (m : ST U)
   (h' : U -> HT V) (k : U -> ST V),
-valid h m -> (forall x, valid (h' x) (k x)) -> valid (hoare_bind h h') (m >>= k).
+valid h m -> (forall x, valid (h' x) (k x)) -> valid (prepost_bind h h') (m >>= k).
 Proof.
 move=> U V h m h' k valid_m valid_k s [Hpr Hpo] v t''.
-rewrite runStateTbind /=.
+rewrite runStateTbind.
 case run_m: runStateT=> [[] | [u t]] //= H.
-(* have post_m : post h s u t := valid_m s Hpr u t run_m. *)
 exists u, t; split.
 - exact: valid_m.
 - apply: valid_k.
@@ -154,8 +152,56 @@ exists u, t; split.
 Qed.
 
 HB.about isMonadHoare.Build.
-HB.about hoare.
+HB.about prepost.
 HB.instance Definition _ := isMonadHoare.Build T option_monad ST HT valid_ret valid_bind.
 
 End vld_s.
 End HoareModel.
+
+Definition wp {T U : UU0} (h : prepost T U) (Q : U -> set T) : set T :=
+  fun s => pre h s /\ forall x s', post h s x s' -> Q x s'.
+
+Section weakest_preconditions.
+Context {T U V : UU0}.
+
+Lemma wp_intro (h : prepost T U) (Q : U -> set T) s
+    (pre_h : pre h s)
+    (post_Q : forall x s', post h s x s' -> Q x s') :
+  wp h Q s.
+Proof. by []. Qed.
+
+Lemma wp_pre (h : prepost T U) (Q : U -> set T) s :
+  wp h Q s -> pre h s.
+
+Admitted.
+
+Lemma wp_post (h : prepost T U) (Q : U -> set T) s x s' :
+  wp h Q s -> post h s x s' -> Q x s'.
+Admitted.
+
+Lemma wp_weaken (h : prepost T U) (Q Q' : U -> set T) s :
+  wp h Q s ->
+  (forall x s', Q x s' -> Q' x s') ->
+  wp h Q' s.
+Admitted.
+
+Lemma wp_prepost_ret (x : U) (Q : U -> set T) s :
+  wp (prepost_ret x) Q s <-> Q x s.
+Admitted.
+
+Lemma wp_prepost_bind (h : prepost T U) (k : U -> prepost T V)
+    (Q : V -> set T) s :
+  wp (prepost_bind h k) Q s <->
+  wp h (fun x s' => wp (k x) Q s') s.
+Admitted.
+
+Lemma wp_ret (x : U) (Q : U -> set T) s :
+  wp (Ret x : prepost T U) Q s <-> Q x s.
+Admitted.
+
+Lemma wp_bind (h : prepost T U) (k : U -> prepost T V)
+    (Q : V -> set T) s :
+  wp (h >>= k) Q s <-> wp h (fun x s' => wp (k x) Q s') s.
+Admitted.
+
+End weakest_preconditions.
